WIP: going total

state/TargetLang.fst
@@ -2,108 +2,38 @@ module TargetLang
 
 open FStar.Tactics
 open FStar.Tactics.Typeclasses
-open FStar.Universe
 
 open Labeled.Monotonic.Heap
 open Labeled.MST
 open Witnessable
 
-unfold let shallowly_contained_low (#a:Type) {| c:witnessable a |} (v:a) (h:lheap) =
-  c.satisfy v h contains_pred /\ c.satisfy v h is_low_pred
-
-unfold let pre_tgt_arrow
-  (#t1:Type) {| c1 : witnessable t1 |}
-  (#inv:lheap -> Type0)
-  (x:t1) (h0:lheap) =
-  inv h0 /\
-  shallowly_contained_low #t1 #c1 x h0
-
-unfold let post_tgt_arrow
-  (#t1:Type) {| c1 : witnessable t1 |}
-  (#t2:Type) {| c2 : witnessable t2 |}
-  (#inv:lheap -> Type0)
-  (x:t1) (h0:lheap) (r:t2) (h1:lheap) =
-  inv h1 /\
-  modifies_only_label Low h0 h1 /\                       (* allows low references to be modified *)
-  modifies_classification Set.empty h0 h1 /\             (* no modifications of the classification *)
-  shallowly_contained_low #t2 #c2 r h1
-
-let mk_tgt_arrow 
-  (inv:lheap -> Type0)
-  (t1:Type) {| c1 : witnessable t1 |}
-  (t2:Type) {| c2 : witnessable t2 |}
-= x:t1 -> ST t2 
-    (requires (pre_tgt_arrow #t1 #c1 #inv x ))
-    (ensures (post_tgt_arrow #t1 #c1 #t2 #c2 #inv x))
-
 (** _elab_typ should be in translation file, but it is here because 
     we need it to write our invariants **)
-open STLC
+type inv_typ =
+  | InvT_Unit
+  | InvT_Nat
+  | InvT_Sum : inv_typ -> inv_typ -> inv_typ
+  | InvT_Pair : inv_typ -> inv_typ -> inv_typ
+  | InvT_Ref : inv_typ -> inv_typ
+  | InvT_LList : inv_typ -> inv_typ
 
-let rec is_base_typ (t:typ) =
+let rec to_Type (t:inv_typ) : Type u#0 = 
   match t with
-  | TUnit -> True
-  | TNat -> True
-  | TSum t1 t2 -> is_base_typ t1 /\ is_base_typ t2
-  | TPair t1 t2 -> is_base_typ t1 /\ is_base_typ t2
-  | TRef t -> is_base_typ t
-  | TLList t -> is_base_typ t
-  | TArr _ _ -> False
+  | InvT_Unit -> unit
+  | InvT_Nat -> int
+  | InvT_Sum t1 t2 -> either (to_Type t1) (to_Type t2)
+  | InvT_Pair t1 t2 -> (to_Type t1) * (to_Type t2)
+  | InvT_Ref t -> ref (to_Type t)
+  | InvT_LList t -> linkedList (to_Type t)
 
-type base_typ = t:typ{is_base_typ t}
-
-let rec elab_typ_base (t:base_typ) : Type u#0 = 
+let rec to_Type_solve (t:inv_typ) : witnessable (to_Type t) =
   match t with
-  | TUnit -> unit
-  | TNat -> int
-  | TSum t1 t2 -> either (elab_typ_base t1) (elab_typ_base t2)
-  | TPair t1 t2 -> (elab_typ_base t1) * (elab_typ_base t2)
-  | TRef t -> ref (elab_typ_base t)
-  | TLList t -> linkedList (elab_typ_base t)
-
-let rec elab_typ_base_tc (t:base_typ) : witnessable (elab_typ_base t) =
-  match t with
-  | TUnit -> witnessable_unit
-  | TNat -> witnessable_int
-  | TSum t1 t2 -> witnessable_sum (elab_typ_base t1) (elab_typ_base t2) #(elab_typ_base_tc t1) #(elab_typ_base_tc t2)
-  | TPair t1 t2 -> witnessable_pair (elab_typ_base t1) (elab_typ_base t2) #(elab_typ_base_tc t1) #(elab_typ_base_tc t2)
-  | TRef t -> witnessable_ref (elab_typ_base t) #(elab_typ_base_tc t)
-  | TLList t -> witnessable_llist (elab_typ_base t) #(elab_typ_base_tc t)
-
-let rec _elab_typ (t:typ) (inv:lheap -> Type0): tt:Type u#1 & witnessable tt =
-  match t with
-  | TArr t1 t2 -> begin
-    let tt1 = _elab_typ t1 inv in
-    let tt2 = _elab_typ t2 inv in
-    (| mk_tgt_arrow inv (dfst tt1) #(dsnd tt1) (dfst tt2) #(dsnd tt2),
-       witnessable_arrow (dfst tt1) (dfst tt2) pre_tgt_arrow post_tgt_arrow
-    |)
-  end 
-  | TUnit -> (| raise_t unit, solve |)
-  | TNat -> (| raise_t int, solve |)
-  | TSum t1 t2 ->
-    let (| tt1, c_tt1 |) = _elab_typ t1 inv in
-    let (| tt2, c_tt2 |) = _elab_typ t2 inv in
-    (| raise_t (either tt1 tt2), witnessable_univ_raise _ #(witnessable_sum tt1 tt2 #c_tt1 #c_tt2) |)
-  | TPair t1 t2 ->
-    let (| tt1, c_tt1 |) = _elab_typ t1 inv in
-    let (| tt2, c_tt2 |) = _elab_typ t2 inv in
-    (| raise_t (tt1 * tt2), witnessable_univ_raise _ #(witnessable_pair tt1 tt2 #c_tt1 #c_tt2) |)
-  | TRef _ ->
-    let tt = elab_typ_base t in
-    let c_tt = elab_typ_base_tc t in
-    (| Universe.raise_t tt, witnessable_univ_raise _ #c_tt |)
-  | _ -> admit ()
-  
-  // | TLList t ->
-  //   let (| tt, c_tt |) = _elab_typ t inv in
-  //   (| linkedList tt, witnessable_llist tt #c_tt |)
-
-let elab_typ (t:typ) (hinv:lheap -> Type0) : Type =
-  dfst (_elab_typ t hinv)
-
-let elab_typ_tc (t:typ) (hinv:lheap -> Type0) : witnessable (elab_typ t hinv)=
-  dsnd (_elab_typ t hinv)
+  | InvT_Unit -> witnessable_unit
+  | InvT_Nat -> witnessable_int
+  | InvT_Sum t1 t2 -> witnessable_sum (to_Type t1) (to_Type t2) #(to_Type_solve t1) #(to_Type_solve t2)
+  | InvT_Pair t1 t2 -> witnessable_pair (to_Type t1) (to_Type t2) #(to_Type_solve t1) #(to_Type_solve t2)
+  | InvT_Ref t -> witnessable_ref (to_Type t) #(to_Type_solve t)
+  | InvT_LList t -> witnessable_llist (to_Type t) #(to_Type_solve t)
 
 let inv_points_to (h:lheap) pred =
   // forall (a:Type) (c:witnessable a) (r:ref a). 
@@ -115,36 +45,35 @@ let inv_points_to (h:lheap) pred =
 
   // however, the following version needs an inversion lemma that cannot be proven in F* yet
   // because one cannot reason about the types of effectful arrows. e.g., `int =!= int -> ST int` cannot be proven
-  (forall (a:typ) (inv:lheap -> Type0) (r:ref (elab_typ a inv)).
-    (witnessable_ref _ #(elab_typ_tc a inv)).satisfy r h pred ==> 
-      (elab_typ_tc a inv).satisfy (sel h r) h pred)
+  (forall (a:inv_typ) (r:ref (to_Type a)).
+    (witnessable_ref _ #(to_Type_solve a)).satisfy r h pred ==> 
+      (to_Type_solve a).satisfy (sel h r) h pred)
 
 let inv_low_contains (h:lheap) = 
   inv_points_to h contains_pred /\ inv_points_to h is_low_pred
 
-
-let eliminate_inv_points_to (h:lheap) (a:typ) (hinv:lheap -> Type0) (r:ref (elab_typ a hinv)) pred :
+let eliminate_inv_points_to (h:lheap) a (r:ref (to_Type a)) pred :
   Lemma
     (requires (inv_points_to h pred))
     (ensures (
-      (witnessable_ref (elab_typ a hinv) #(elab_typ_tc a hinv)).satisfy r h pred ==> 
-        (elab_typ_tc a hinv).satisfy (sel h r) h pred
+      (witnessable_ref (to_Type a) #(to_Type_solve a)).satisfy r h pred ==> 
+        (to_Type_solve a).satisfy (sel h r) h pred
     )) = ()
 
-let eliminate_inv_low (h:lheap) (a:typ) (hinv:lheap -> Type0) (r:ref (elab_typ a hinv)) :
+let eliminate_inv_low h a (r:ref (to_Type a)) :
   Lemma
     (requires (inv_points_to h is_low_pred))
     (ensures (
-      (witnessable_ref (elab_typ a hinv) #(elab_typ_tc a hinv)).satisfy r h is_low_pred ==> 
-        (elab_typ_tc a hinv).satisfy (sel h r) h is_low_pred
+      (witnessable_ref (to_Type a) #(to_Type_solve a)).satisfy r h is_low_pred ==> 
+        (to_Type_solve a).satisfy (sel h r) h is_low_pred
     )) = ()
 
-let eliminate_inv_contains (h:lheap) (a:typ) (hinv:lheap -> Type0) (r:ref (elab_typ a hinv)) :
+let eliminate_inv_contains h a (hinv:lheap -> Type0) (r:ref (to_Type a)) :
   Lemma
     (requires (inv_points_to h contains_pred))
     (ensures (
-      (witnessable_ref (elab_typ a hinv) #(elab_typ_tc a hinv)).satisfy r h contains_pred ==> 
-        (elab_typ_tc a hinv).satisfy (sel h r) h contains_pred
+      (witnessable_ref (to_Type a) #(to_Type_solve a)).satisfy r h contains_pred ==> 
+        (to_Type_solve a).satisfy (sel h r) h contains_pred
     )) = ()
 
 effect IST (a:Type) (pre:st_pre) (post: (h:lheap -> Tot (st_post' a (pre h)))) =
@@ -152,3 +81,255 @@ effect IST (a:Type) (pre:st_pre) (post: (h:lheap -> Tot (st_post' a (pre h)))) =
     (requires (fun h0      -> inv_low_contains h0 /\ pre h0))
     (ensures  (fun h0 r h1 -> inv_low_contains h1 /\ post h0 r h1))
 
+let rec inversion (a:inv_typ) (xa:inv_typ) :
+  Lemma
+    (requires (to_Type a == to_Type xa))
+    (ensures (a == xa /\ to_Type_solve a == to_Type_solve xa)) =
+  match a with
+  | InvT_Unit -> ()
+  | InvT_Nat -> ()
+  | InvT_Sum t1 t2 -> begin
+    let InvT_Sum t1' t2' = xa in
+    assume (forall a b c d. either a b == either c d ==> a == c /\ b == d);
+    inversion t1 t1';
+    inversion t2 t2'
+  end
+  | InvT_Pair t1 t2 -> begin
+    let InvT_Pair t1' t2' = xa in
+    assume (forall a b c d. (a * b) == (c * d) ==> a == c /\ b == d);
+    inversion t1 t1';
+    inversion t2 t2'
+  end
+  | InvT_Ref t -> begin
+    let InvT_Ref t' = xa in
+    assume (forall a b. ref a == ref b ==> a == b);
+    inversion t t'
+  end
+  | InvT_LList t -> begin
+    let InvT_LList t' = xa in
+    assume (forall a b. linkedList a == linkedList b ==> a == b);
+    inversion t t'
+  end
+  
+let lemma_write_preserves_is_low t (x:ref (to_Type t)) (v:to_Type t) (h0 h1:lheap) : Lemma
+  (requires (
+    h0 `lheap_rel` h1 /\
+    equal_dom h0 h1 /\
+    modifies (Set.singleton (addr_of x)) h0 h1 /\
+    modifies_classification Set.empty h0 h1 /\
+    sel h1 x == v /\
+    (to_Type_solve (InvT_Ref t)).satisfy x h0 is_low_pred /\
+    (to_Type_solve t).satisfy v h0 is_low_pred /\
+    inv_points_to h0 is_low_pred))
+  (ensures (
+    inv_points_to h1 is_low_pred)) = 
+  introduce forall a (r:ref (to_Type a)).
+      (witnessable_ref _ #(to_Type_solve a)).satisfy r h1 is_low_pred ==> 
+        (to_Type_solve a).satisfy (sel h1 r) h1 is_low_pred
+  with begin
+    introduce (witnessable_ref _ #(to_Type_solve a)).satisfy r h1 is_low_pred 
+      ==> (to_Type_solve a).satisfy (sel h1 r) h1 is_low_pred
+    with _. begin
+      introduce addr_of r =!= addr_of x ==> (to_Type_solve a).satisfy (sel h1 r) h1 is_low_pred with _. begin
+        eliminate_inv_points_to h0 a r is_low_pred;
+        (to_Type_solve a).satisfy_monotonic (sel h0 r) is_low_pred h0 h1
+      end;
+      introduce addr_of r == addr_of x ==> (to_Type_solve a).satisfy (sel h1 r) h1 is_low_pred with _. begin
+        assert (sel h1 x == v);
+        lemma_sel_same_addr' h1 x r;
+        inversion a t;
+        assert ((to_Type_solve t).satisfy v h0 is_low_pred);
+        (to_Type_solve t).satisfy_monotonic v is_low_pred h0 h1;
+        assert ((to_Type_solve t).satisfy v h1 is_low_pred)
+      end
+    end
+  end
+
+let lemma_write_preserves_contains t (x:ref (to_Type t)) (v:to_Type t) (h0 h1:lheap) : Lemma
+  (requires (
+    h0 `lheap_rel` h1 /\
+    equal_dom h0 h1 /\
+    modifies (Set.singleton (addr_of x)) h0 h1 /\
+    modifies_classification Set.empty h0 h1 /\
+    sel h1 x == v /\
+    (to_Type_solve (InvT_Ref t)).satisfy x h0 contains_pred /\
+    (to_Type_solve t).satisfy v h0 contains_pred /\
+    inv_points_to h0 contains_pred))
+  (ensures (
+    inv_points_to h1 contains_pred)) = 
+  introduce forall a (r:ref (to_Type a)).
+      (witnessable_ref _ #(to_Type_solve a)).satisfy r h1 contains_pred ==> 
+        (to_Type_solve a).satisfy (sel h1 r) h1 contains_pred
+  with begin
+    introduce (witnessable_ref _ #(to_Type_solve a)).satisfy r h1 contains_pred 
+      ==> (to_Type_solve a).satisfy (sel h1 r) h1 contains_pred
+    with _. begin
+      introduce addr_of r =!= addr_of x ==> (to_Type_solve a).satisfy (sel h1 r) h1 contains_pred with _. begin
+        eliminate_inv_points_to h0 a r contains_pred;
+        (to_Type_solve a).satisfy_monotonic (sel h0 r) contains_pred h0 h1
+      end;
+      introduce addr_of r == addr_of x ==> (to_Type_solve a).satisfy (sel h1 r) h1 contains_pred with _. begin
+        assert (sel h1 x == v);
+        lemma_sel_same_addr' h1 x r;
+        inversion a t;
+        assert ((to_Type_solve t).satisfy v h0 contains_pred);
+        (to_Type_solve t).satisfy_monotonic v contains_pred h0 h1;
+        assert ((to_Type_solve t).satisfy v h1 contains_pred)
+      end
+    end
+  end
+
+
+let lemma_declassify_preserves_contains t (x:ref (to_Type t)) (h0 h1:lheap) : Lemma
+  (requires (
+    modifies_none h0 h1 /\
+    h0 `lheap_rel` h1 /\
+    equal_dom h0 h1 /\
+    modifies_classification (only x) h0 h1 /\
+    (to_Type_solve (InvT_Ref t)).satisfy x h0 contains_pred /\ 
+    (to_Type_solve t).satisfy (sel h0 x) h0 contains_pred /\
+    inv_points_to h0 contains_pred))
+  (ensures (inv_points_to h1 contains_pred)) =
+  introduce forall a (r:ref (to_Type a)).
+      (witnessable_ref _ #(to_Type_solve a)).satisfy r h1 contains_pred ==> 
+        (to_Type_solve a).satisfy (sel h1 r) h1 contains_pred
+  with begin
+    let refw = witnessable_ref _ #(to_Type_solve a) in
+    introduce refw.satisfy r h1 contains_pred ==> (to_Type_solve a).satisfy (sel h1 r) h1 contains_pred
+    with _. begin
+      introduce refw.satisfy r h0 contains_pred ==> (to_Type_solve a).satisfy (sel h1 r) h1 contains_pred
+      with _. (to_Type_solve a).satisfy_monotonic (sel h0 r) contains_pred h0 h1;
+      
+      introduce ~(refw.satisfy r h0 contains_pred) ==> (to_Type_solve a).satisfy (sel h1 r) h1 contains_pred
+      with _. begin
+        assert (addr_of r == addr_of x);
+        lemma_sel_same_addr' h1 x r;
+        assert (to_Type_solve a == to_Type_solve t);
+        inversion a t;
+        assert (to_Type_solve a == to_Type_solve t);
+
+        assert ((to_Type_solve t).satisfy (sel h0 x) h0 contains_pred);
+        (to_Type_solve t).satisfy_monotonic (sel h0 x) contains_pred h0 h1;
+        assert (sel h0 x == sel h1 x);
+        assert ((to_Type_solve t).satisfy (sel h1 x) h1 contains_pred);
+        assert ((to_Type_solve a).satisfy (sel h1 r) h1 contains_pred)
+      end
+    end
+  end
+
+let lemma_declassify_preserves_is_low t (x:ref (to_Type t)) (h0 h1:lheap) : Lemma
+  (requires (
+    modifies_none h0 h1 /\
+    h0 `lheap_rel` h1 /\
+    equal_dom h0 h1 /\
+    modifies_classification (only x) h0 h1 /\
+    (to_Type_solve (InvT_Ref t)).satisfy x h1 is_low_pred /\
+    (to_Type_solve t).satisfy (sel h0 x) h0 is_low_pred /\
+    inv_points_to h0 is_low_pred))
+  (ensures (inv_points_to h1 is_low_pred)) =
+  introduce forall a (inv:lheap -> Type0) (r:ref (to_Type a)).
+      (witnessable_ref _ #(to_Type_solve a)).satisfy r h1 is_low_pred ==> 
+        (to_Type_solve a).satisfy (sel h1 r) h1 is_low_pred
+  with begin
+    let refw = witnessable_ref _ #(to_Type_solve a) in
+    introduce refw.satisfy r h1 is_low_pred ==> (to_Type_solve a).satisfy (sel h1 r) h1 is_low_pred
+    with _. begin
+      introduce refw.satisfy r h0 is_low_pred ==> (to_Type_solve a).satisfy (sel h1 r) h1 is_low_pred
+      with _. (to_Type_solve a).satisfy_monotonic (sel h0 r) is_low_pred h0 h1;
+      
+      introduce ~(refw.satisfy r h0 is_low_pred) ==> (to_Type_solve a).satisfy (sel h1 r) h1 is_low_pred
+      with _. begin
+        assert (addr_of r == addr_of x);
+        lemma_sel_same_addr' h1 x r;
+        inversion a t;
+        (to_Type_solve t).satisfy_monotonic (sel h0 x) is_low_pred h0 h1
+      end
+    end
+  end
+
+let lemma_ist_alloc_preserves_contains t (x:ref (to_Type t)) (v:to_Type t) (h0 h1:lheap) : Lemma
+  (requires (
+    h0 `lheap_rel` h1 /\
+    h1 == upd h0 x v /\ 
+    fresh x h0 h1 /\ 
+    modifies Set.empty h0 h1 /\
+    modifies_classification Set.empty h0 h1 /\
+    sel h1 x == v /\ 
+    label_of x h1 == High /\
+    is_mm x == false /\
+    (to_Type_solve t).satisfy v h0 contains_pred /\
+    inv_points_to h0 contains_pred))
+  (ensures (
+    inv_points_to h1 contains_pred)) = 
+  introduce forall a (r:ref (to_Type a)).
+      (witnessable_ref _ #(to_Type_solve a)).satisfy r h1 contains_pred ==> 
+        (to_Type_solve a).satisfy (sel h1 r) h1 contains_pred
+  with begin
+    introduce (witnessable_ref _ #(to_Type_solve a)).satisfy r h1 contains_pred 
+      ==> (to_Type_solve a).satisfy (sel h1 r) h1 contains_pred
+    with _. begin
+      introduce addr_of r =!= addr_of x ==> (to_Type_solve a).satisfy (sel h1 r) h1 contains_pred with _. begin
+        eliminate_inv_points_to h0 a r contains_pred;
+        assert (h0 `contains` r);
+        (to_Type_solve a).satisfy_monotonic (sel h0 r) contains_pred h0 h1
+      end;
+      introduce addr_of r == addr_of x ==> (to_Type_solve a).satisfy (sel h1 r) h1 contains_pred with _. begin
+        assert (sel h1 x == v);
+        lemma_sel_same_addr' h1 x r;
+        inversion a t;
+        (to_Type_solve t).satisfy_monotonic v contains_pred h0 h1
+      end
+    end
+  end
+
+let lemma_ist_alloc_preserves_is_low t (x:ref (to_Type t)) (v:to_Type t) (h0 h1:lheap) : Lemma
+  (requires (
+    h0 `lheap_rel` h1 /\
+    h1 == upd h0 x v /\ 
+    fresh x h0 h1 /\ 
+    modifies Set.empty h0 h1 /\
+    modifies_classification Set.empty h0 h1 /\
+    sel h1 x == v /\ 
+    label_of x h1 == High /\
+    is_mm x == false /\
+    (to_Type_solve t).satisfy v h0 contains_pred /\
+    inv_points_to h0 is_low_pred))
+  (ensures (
+    inv_points_to h1 is_low_pred)) = 
+  introduce forall a (r:ref (to_Type a)).
+      (witnessable_ref _ #(to_Type_solve a)).satisfy r h1 is_low_pred ==> 
+        (to_Type_solve a).satisfy (sel h1 r) h1 is_low_pred
+  with begin
+    introduce (witnessable_ref _ #(to_Type_solve a)).satisfy r h1 is_low_pred 
+      ==> (to_Type_solve a).satisfy (sel h1 r) h1 is_low_pred
+    with _. begin
+      introduce addr_of r =!= addr_of x ==> (to_Type_solve a).satisfy (sel h1 r) h1 is_low_pred with _. begin
+        eliminate_inv_points_to h0 a r is_low_pred;
+        assert (h0 `contains` r);
+        (to_Type_solve a).satisfy_monotonic (sel h0 r) is_low_pred h0 h1;
+        assert ((to_Type_solve a).satisfy (sel h1 r) h1 is_low_pred)
+      end;
+      introduce addr_of r == addr_of x ==> (to_Type_solve a).satisfy (sel h1 r) h1 is_low_pred with _. begin
+        assert (sel h1 x == v);
+        lemma_sel_same_addr' h1 x r;
+        assert (label_of r h1 == Low);
+        assert (label_of x h1 == High);
+        assert (r == x);
+        assert False
+      end
+    end
+  end
+
+
+let ist_alloc (#t:inv_typ) (init:to_Type t)
+: IST (ref (to_Type t))
+    (fun h -> 
+      (to_Type_solve t).satisfy init h contains_pred)
+    (alloc_post #(to_Type t) init)
+=
+  let h0 = get () in
+  let r = alloc init in
+  let h1 = get () in
+  lemma_ist_alloc_preserves_contains t r init h0 h1;
+  lemma_ist_alloc_preserves_is_low t r init h0 h1;
+  r
